CredibleCompilation/CSEOpt.lean
@@ -58,8 +58,7 @@ def exprRefsVar (e : Expr) (x : Var) : Bool :=
   | .fbin _ a b => exprRefsVar a x || exprRefsVar b x
   | .intToFloat a => exprRefsVar a x
   | .floatToInt a => exprRefsVar a x
-  | .floatExp a   => exprRefsVar a x
-  | .floatSqrt a  => exprRefsVar a x
+  | .floatUnary _ a => exprRefsVar a x
   | .lit _     => false
   | .blit _    => false
   | .flit _    => false
@@ -117,8 +116,7 @@ def transfer (avail : AvailSet) (instr : TAC) : AvailSet :=
   | .arrLoad x _ _ _   => killVar avail x
   | .intToFloat x _    => killVar avail x
   | .floatToInt x _    => killVar avail x
-  | .floatExp x _      => killVar avail x
-  | .floatSqrt x _     => killVar avail x
+  | .floatUnary x _ _  => killVar avail x
   | _ => avail
 
 -- ============================================================
