CredibleCompilation/RefCompiler/Defs.lean
@@ -316,19 +316,12 @@ theorem FragExec.single_floatToInt {p : Prog} {pc : Nat} {σ : Store} {am : Arra
     FragExec p pc σ (pc + 1) (σ[x ↦ .int (floatToIntBv f)]) am am :=
   Steps.single (Step.floatToInt h hy)
 
-theorem FragExec.single_floatExp {p : Prog} {pc : Nat} {σ : Store} {am : ArrayMem}
-    {x y : Var} {f : BitVec 64}
-    (h : p[pc]? = some (.floatExp x y))
+theorem FragExec.single_floatUnary {p : Prog} {pc : Nat} {σ : Store} {am : ArrayMem}
+    {x y : Var} {op : FloatUnaryOp} {f : BitVec 64}
+    (h : p[pc]? = some (.floatUnary x op y))
     (hy : σ y = .float f) :
-    FragExec p pc σ (pc + 1) (σ[x ↦ .float (floatExpBv f)]) am am :=
-  Steps.single (Step.floatExp h hy)
-
-theorem FragExec.single_floatSqrt {p : Prog} {pc : Nat} {σ : Store} {am : ArrayMem}
-    {x y : Var} {f : BitVec 64}
-    (h : p[pc]? = some (.floatSqrt x y))
-    (hy : σ y = .float f) :
-    FragExec p pc σ (pc + 1) (σ[x ↦ .float (floatSqrtBv f)]) am am :=
-  Steps.single (Step.floatSqrt h hy)
+    FragExec p pc σ (pc + 1) (σ[x ↦ .float (op.eval f)]) am am :=
+  Steps.single (Step.floatUnary h hy)
 
 theorem FragExec.single_arrStore_float {p : Prog} {pc : Nat} {σ : Store} {am : ArrayMem}
     {arr : ArrayName} {idx val : Var} {idxVal v : BitVec 64}
